need to find a way to make sure my asserts work

Assignment1/Ex7.dfy
@@ -5,6 +5,10 @@
 //				   September 2019						   //
 /////////////////////////////////////////////////////////////
 
+// functions were used to allow for my specification to have 
+// functional behaviour e.g. counting
+// link to resource: https://www.engr.mun.ca/~theo/Courses/AlgCoCo/6892-downloads/dafny-notes-010.pdf
+
 // Ex7.dfy 10 marks. 
 // Write a Dafny method Just1;
 // This method should return true if and only if the array contains just one instance of the key. 
@@ -28,10 +32,10 @@
 
 method Just1(a: array<int>, key: int) returns (b: bool)
 requires a != null
-ensures VerifyJustOne(a, key) ==> b
-ensures !VerifyJustOne(a, key) ==> !b
-ensures b ==> VerifyJustOne(a, key)
-ensures !b ==> !VerifyJustOne(a, key)
+ensures (a.Length > 0 && (CountOccurencesFromZeroToIndex(a, key, a.Length - 1) == 1)) ==> b
+ensures !(a.Length > 0 && (CountOccurencesFromZeroToIndex(a, key, a.Length - 1) == 1)) ==> !b
+ensures b ==>  a.Length > 0 &&(CountOccurencesFromZeroToIndex(a, key, a.Length - 1) == 1)
+ensures !b ==>  !(a.Length > 0 &&(CountOccurencesFromZeroToIndex(a, key, a.Length - 1) == 1))
 ensures forall i :: 0 <= i < a.Length ==> a[i] == old(a[i])
 {
 
@@ -39,8 +43,8 @@ ensures forall i :: 0 <= i < a.Length ==> a[i] == old(a[i])
     var count := 0;
     while i < a.Length
     invariant 0 <= i <= a.Length
-    invariant count == 1 <==> ((exists j :: 0 <=  j < i && a[j] == key) &&
-                (forall j,k :: 0 <= j <= k < i && (a[j] == a[k]) && (a[j] == key) ==> (j == k)))
+    invariant i > 0 ==> count == CountOccurencesFromZeroToIndex(a, key, i-1)
+    invariant i == 0 ==> count == 0
     {
         if(a[i] == key)
         {
@@ -59,6 +63,29 @@ reads a;
     (forall i,j :: 0 <= i <= j < a.Length && (a[i] == a[j]) && (a[i] == key) ==> i == j)
 }
 
+function CountOccurencesFromZeroToIndex(a: array<int>, key: int, maxIndex: int): int
+requires a != null
+requires maxIndex >= 0
+requires maxIndex < a.Length
+reads a
+// here i supply my variant that maxIndex is decreasing
+decreases maxIndex
+{
+    if maxIndex == 0 
+    then
+        if(a[maxIndex] == key) 
+        then 
+            1
+        else
+            0
+    else
+        if a[maxIndex] == key 
+        then
+            CountOccurencesFromZeroToIndex(a, key, maxIndex - 1) + 1
+        else
+            CountOccurencesFromZeroToIndex(a, key, maxIndex - 1) 
+}
+
 method Main()
 {
     var testArray1: array<int> := new int[4];
@@ -73,49 +100,55 @@ method Main()
     assert testArray1[2] == 2;
     assert testArray1[3] == 1;
     var test1 := Just1(testArray1, 1);
+    assert CountOccurencesFromZeroToIndex(testArray1, 1, testArray1.Length - 1) == 3;
     assert !VerifyJustOne(testArray1, 1);
-    // assert !test1;
-    // assert !VerifyJustOne(testArray1, 1) && !test1;
+    assert !test1;
+    assert !VerifyJustOne(testArray1, 1) && !test1;
 
     assert testArray1.Length == 4;
     assert testArray1[0] == 1;
     assert testArray1[1] == 1;
     assert testArray1[2] == 2;
     assert testArray1[3] == 1;
-    var test2 := Just1(testArray1, 2);
+     var test2 := Just1(testArray1, 2);
+    assert CountOccurencesFromZeroToIndex(testArray1, 2, testArray1.Length - 1) == 1;
     assert VerifyJustOne(testArray1, 2);
-    // assert test2;
-    // assert VerifyJustOne(testArray1, 2) && test2;
+    assert test2;
+    assert VerifyJustOne(testArray1, 2) && test2;
     
     assert testArray1.Length == 4;
     assert testArray1[0] == 1;
     assert testArray1[1] == 1;
     assert testArray1[2] == 2;
     assert testArray1[3] == 1;
-    var test3 := Just1(testArray1, 3);
+     var test3 := Just1(testArray1, 3);
+    assert CountOccurencesFromZeroToIndex(testArray1, 3, testArray1.Length - 1) == 0;
     assert !VerifyJustOne(testArray1, 3);
-    // assert !test3;
-    // assert !VerifyJustOne(testArray1, 3) && test3;
+    assert !test3;
+    assert !VerifyJustOne(testArray1, 3) && test3;
 
     assert testArray2.Length == 1;
     assert testArray2[0] == 1;
-    var test4 := Just1(testArray2, 1);
+     var test4 := Just1(testArray2, 1);
+    assert CountOccurencesFromZeroToIndex(testArray2, 1, testArray2.Length - 1) == 1;
     assert VerifyJustOne(testArray2, 1);
-    // assert test4;
-    // assert VerifyJustOne(testArray2, 1) && test4;
+    assert test4;
+    assert VerifyJustOne(testArray2, 1) && test4;
 
     assert testArray2.Length == 1;
     assert testArray2[0] == 1;
-    var test5 := Just1(testArray2, 2);
+     var test5 := Just1(testArray2, 2);
+    assert CountOccurencesFromZeroToIndex(testArray2, 2, testArray2.Length - 1) == 0;
     assert !VerifyJustOne(testArray2, 2);
-    // assert !test5;
-    // assert !VerifyJustOne(testArray2, 2) && !test5;
+    assert !test5;
+    assert !VerifyJustOne(testArray2, 2) && !test5;
 
     assert testArray3.Length == 0;
-    var test6 := Just1(testArray3, 1);
+     var test6 := Just1(testArray3, 1);
+    assert CountOccurencesFromZeroToIndex(testArray3, 1, testArray1.Length) == 0;
     assert !VerifyJustOne(testArray3, 1);
-    // assert !test6;
-    // assert !VerifyJustOne(testArray3, 1) && !test6;
+    assert !test6;
+    assert !VerifyJustOne(testArray3, 1) && !test6;
 
     print test1, "\n", test2, "\n", test3, "\n", test4, "\n", test5, "\n", test6, "\n";
 }
